Add several more builtin operators
Not all are implemented in the semantics yet. Also the cv translation of
some of the int operations is just something to get it to work, probably
not actually good.

vyperInterpreterScript.sml
@@ -1,12 +1,126 @@
 open HolKernel boolLib bossLib Parse wordsLib blastLib dep_rewrite monadsyntax
      alistTheory rich_listTheory byteTheory finite_mapTheory
-     arithmeticTheory combinTheory pairTheory whileTheory
+     int_bitwiseTheory arithmeticTheory combinTheory pairTheory whileTheory
      cv_typeTheory cv_stdTheory cv_transLib
 open vfmTypesTheory vfmStateTheory vyperAstTheory
 
 val () = new_theory "vyperInterpreter";
 
 (* TODO: move *)
+
+val int_exp_pre_def = cv_auto_trans_pre integerTheory.int_exp;
+
+Theorem int_exp_pre[cv_pre]:
+  int_exp_pre p v
+Proof
+  qid_spec_tac`p`
+  \\ Induct_on `v`
+  \\ rw[Once int_exp_pre_def]
+QED
+
+(* TODO: I don't know if this is the best way to translate this... *)
+val () = cv_auto_trans num_of_bits_def;
+val () = cv_auto_trans int_of_bits_def;
+val () = cv_auto_trans bits_of_int_def;
+
+Definition bits_bitwise_and_def:
+  bits_bitwise_and = bits_bitwise $/\
+End
+
+val bits_bitwise_and_pre_def = bits_bitwise_def
+ |> oneline
+ |> Q.GEN`f`
+ |> Q.ISPEC`$/\`
+ |> SRULE [GSYM bits_bitwise_and_def]
+ |> (curry $ flip $ uncurry cv_trans_pre_rec)
+    (WF_REL_TAC `inv_image ($< LEX $<) (λ(x,y). (cv_size x, cv_size y))`
+     \\ rw[]
+     \\ Cases_on`cv_v` \\ gvs[]
+     \\ Cases_on`cv_v0` \\ gvs[]
+     \\ qmatch_assum_rename_tac`_ (cv_ispair p)`
+     \\ Cases_on`p` \\ gvs[]
+     \\ qmatch_assum_rename_tac`_ (cv_ispair p)`
+     \\ Cases_on`p` \\ gvs[]);
+
+Theorem bits_bitwise_and_pre[cv_pre]:
+  ∀x y. bits_bitwise_and_pre x y
+Proof
+  simp[FORALL_PROD]
+  \\ qid_spec_tac`f:bool -> bool -> bool`
+  \\ ho_match_mp_tac bits_bitwise_ind
+  \\ rw[]
+  \\ rw[Once bits_bitwise_and_pre_def]
+QED
+
+val () = int_and_def
+  |> SRULE [FUN_EQ_THM, int_bitwise_def, GSYM bits_bitwise_and_def]
+  |> cv_trans;
+
+Definition bits_bitwise_or_def:
+  bits_bitwise_or = bits_bitwise $\/
+End
+
+val bits_bitwise_or_pre_def = bits_bitwise_def
+ |> oneline
+ |> Q.GEN`f`
+ |> Q.ISPEC`$\/`
+ |> SRULE [GSYM bits_bitwise_or_def]
+ |> (curry $ flip $ uncurry cv_trans_pre_rec)
+    (WF_REL_TAC `inv_image ($< LEX $<) (λ(x,y). (cv_size x, cv_size y))`
+     \\ rw[]
+     \\ Cases_on`cv_v` \\ gvs[]
+     \\ Cases_on`cv_v0` \\ gvs[]
+     \\ qmatch_assum_rename_tac`_ (cv_ispair p)`
+     \\ Cases_on`p` \\ gvs[]
+     \\ qmatch_assum_rename_tac`_ (cv_ispair p)`
+     \\ Cases_on`p` \\ gvs[]);
+
+Theorem bits_bitwise_or_pre[cv_pre]:
+  ∀x y. bits_bitwise_or_pre x y
+Proof
+  simp[FORALL_PROD]
+  \\ qid_spec_tac`f:bool -> bool -> bool`
+  \\ ho_match_mp_tac bits_bitwise_ind
+  \\ rw[]
+  \\ rw[Once bits_bitwise_or_pre_def]
+QED
+
+val () = int_or_def
+  |> SRULE [FUN_EQ_THM, int_bitwise_def, GSYM bits_bitwise_or_def]
+  |> cv_trans;
+
+Definition bits_bitwise_xor_def:
+  bits_bitwise_xor = bits_bitwise ((≠) : bool -> bool -> bool)
+End
+
+val bits_bitwise_xor_pre_def = bits_bitwise_def
+ |> oneline
+ |> Q.GEN`f`
+ |> Q.ISPEC`λx:bool y. x ≠ y`
+ |> SRULE [GSYM bits_bitwise_xor_def]
+ |> (curry $ flip $ uncurry cv_trans_pre_rec)
+    (WF_REL_TAC `inv_image ($< LEX $<) (λ(x,y). (cv_size x, cv_size y))`
+     \\ rw[]
+     \\ Cases_on`cv_v` \\ gvs[]
+     \\ Cases_on`cv_v0` \\ gvs[]
+     \\ qmatch_assum_rename_tac`_ (cv_ispair p)`
+     \\ Cases_on`p` \\ gvs[]
+     \\ qmatch_assum_rename_tac`_ (cv_ispair p)`
+     \\ Cases_on`p` \\ gvs[]);
+
+Theorem bits_bitwise_xor_pre[cv_pre]:
+  ∀x y. bits_bitwise_xor_pre x y
+Proof
+  simp[FORALL_PROD]
+  \\ qid_spec_tac`f:bool -> bool -> bool`
+  \\ ho_match_mp_tac bits_bitwise_ind
+  \\ rw[]
+  \\ rw[Once bits_bitwise_xor_pre_def]
+QED
+
+val () = int_xor_def
+  |> SRULE [FUN_EQ_THM, int_bitwise_def, GSYM bits_bitwise_xor_def]
+  |> cv_trans;
 
 Theorem INDEX_OF_pre[cv_pre]:
   INDEX_OF_pre x y
@@ -337,6 +451,16 @@ Definition evaluate_binop_def:
   evaluate_binop Mul (IntV i1) (IntV i2) = INL (IntV (i1 * i2)) ∧
   evaluate_binop Div (IntV i1) (IntV i2) = (if i2 = 0 then INR "Div0" else INL (IntV (i1 / i2))) ∧
   evaluate_binop Mod (IntV i1) (IntV i2) = (if i2 = 0 then INR "Mod0" else INL (IntV (i1 % i2))) ∧
+  evaluate_binop Exp (IntV i1) (IntV i2) = (if i2 < 0 then INR "Exp~"
+                                            else INL (IntV (i1 ** (Num i2)))) ∧
+  evaluate_binop And (IntV i1) (IntV i2) = INL (IntV (int_and i1 i2)) ∧
+  evaluate_binop  Or (IntV i1) (IntV i2) = INL (IntV (int_or i1 i2)) ∧
+  evaluate_binop XOr (IntV i1) (IntV i2) = INL (IntV (int_xor i1 i2)) ∧
+  evaluate_binop And (BoolV b1) (BoolV b2) = INL (BoolV (b1 ∧ b2)) ∧
+  evaluate_binop  Or (BoolV b1) (BoolV b2) = INL (BoolV (b1 ∨ b2)) ∧
+  evaluate_binop XOr (BoolV b1) (BoolV b2) = INL (BoolV (b1 ≠ b2)) ∧
+  (* TODO: shifts *)
+  (* TODO: in *)
   evaluate_binop _ _ _ = INR "binop"
 End
 
@@ -376,6 +500,8 @@ Definition evaluate_builtin_def:
   evaluate_builtin cx _ Eq  [IntV i1; IntV i2] = INL (BoolV (i1 = i2)) ∧
   evaluate_builtin cx _ Lt  [IntV i1; IntV i2] = INL (BoolV (i1 < i2)) ∧
   evaluate_builtin cx _ Not [BoolV b] = INL (BoolV (¬b)) ∧
+  evaluate_builtin cx _ Not [IntV i] =
+    (if 0 ≤ i then INL (IntV (int_not i)) else INR "signed Not") ∧
   evaluate_builtin cx _ (Bop bop) [v1; v2] = evaluate_binop bop v1 v2 ∧
   evaluate_builtin cx _ (Msg Sender) [] = INL $ AddressV cx.txn.sender ∧
   evaluate_builtin cx _ (Msg SelfAddr) [] = INL $ AddressV cx.txn.target ∧
